HoldEquivalence.v
@@ -1,0 +1,674 @@
+Require Import Morphisms.
+Require Import Coq.FSets.FMapPositive.
+Require Import List.
+Require Import Rustre.Common.
+Require Import Rustre.DataflowSyntax.
+Require Import Rustre.DataflowListSemantics.
+
+
+Set Implicit Arguments.
+
+
+Ltac inv H := inversion H; subst; clear H.
+
+
+Lemma nth_nil : forall {A} (d : A) n, nth n nil d = d.
+Proof. intros A d [| n]; reflexivity. Qed.
+
+Lemma nth_hd : forall {A} (d : A) l, nth 0 l d = hd d l.
+Proof. intros A d l. now destruct l. Qed.
+
+Lemma nth_last : forall {A} (d : A) l, nth (length l - 1) l d = last l d.
+Proof.
+intros A d l. induction l.
+- simpl. reflexivity.
+- destruct l; trivial. simpl in *. rewrite <- IHl, <- Minus.minus_n_O. reflexivity.
+Qed.
+
+Lemma nth_not_default_lt_length : forall {A} (d : A) n l, nth n l d <> d -> n < length l.
+Proof.
+intros A d n l Heq. destruct (Compare_dec.le_lt_dec (length l) n).
+- elim Heq. now apply nth_overflow.
+- assumption.
+Qed.
+
+Lemma Forall_compat {A} : Proper ((eq ==> iff) ==> eq ==> iff) (@Forall A).
+Proof.
+intros P Q HPQ ? l ?. subst. induction l as [| e l].
+* intuition.
+* split; intro He.
+  + inversion_clear He. constructor.
+    - now apply (HPQ _ _ (reflexivity e)).
+    - now rewrite <- IHl.
+  + inversion_clear He. constructor.
+    - now apply <- (HPQ _ _ (reflexivity e)).
+    - now rewrite IHl.
+Qed.
+
+Lemma find_None_not_In : forall (x : ident) (env : venv), PositiveMap.find x env = None <-> ~PositiveMap.In x env.
+Proof.
+intros x env. split; intro Habs.
++ intros [v Hin]. apply PositiveMap.find_1 in Hin. rewrite Hin in Habs. discriminate.
++ destruct (PositiveMap.find x env) eqn:Hin; trivial. elim Habs. exists v. now apply PositiveMap.find_2.
+Qed.
+
+(** **  The [hold] operator in histories that removes [abs] by keeping the last value **)
+
+Definition update_binding (x : ident) v1 (env : venv) : value :=
+  match v1 with
+    | here _ => v1
+    | abs => 
+        match PositiveMap.find x env with
+          | None => abs
+          | Some v2 => v2
+        end
+  end.
+
+Definition hold_env (curr prev : venv) : venv :=
+  PositiveMap.mapi (fun x v => update_binding x v prev) curr.
+
+(** Hold operator on reverse lists: the first element is the latest (time-wise). *)
+
+Definition hold (h : history) : history :=
+  List.fold_right (fun e l => hold_env e (hd (PositiveMap.empty _) l) :: l) nil h.
+
+(** ***  Lemmas about [update_binding]  **)
+
+Lemma update_in : forall (x : ident) v env, update_binding x (here v) env = here v.
+Proof. reflexivity. Qed.
+
+Lemma update_out : forall (x : ident) v (env : venv),
+  PositiveMap.find x env = Some v -> update_binding x abs env = v.
+Proof. intros x v env Henv. simpl. now rewrite Henv. Qed.
+
+Lemma update_same_none : forall (x : ident) (env e : venv),
+  PositiveMap.find x env = None -> update_binding x abs env = abs.
+Proof. intros x env e Henv. simpl. now rewrite Henv. Qed.
+
+(** ***  Lemmas about [hold_env]  **)
+
+Lemma hold_env_in : forall (curr prev : venv) (x : ident) v,
+  PositiveMap.find x curr = Some (here v) ->
+  PositiveMap.find x (hold_env curr prev) = Some (here v).
+Proof. intros curr prev x v Hcurr. unfold hold_env. rewrite PositiveMap.gmapi, Hcurr. simpl. reflexivity. Qed.
+
+Lemma hold_env_out : forall (curr prev : venv) (x : ident) v,
+  PositiveMap.find x curr = Some abs ->
+  PositiveMap.find x prev = Some v ->
+  PositiveMap.find x (hold_env curr prev) = Some v.
+Proof.
+intros curr prev x v Hcurr Hprev. unfold hold_env.
+rewrite PositiveMap.gmapi, Hcurr. simpl. now rewrite Hprev.
+Qed.
+
+Lemma hold_env_none : forall (curr prev : venv) (x : ident),
+  PositiveMap.find x curr = Some abs ->
+  PositiveMap.find x prev = None ->
+  PositiveMap.find x (hold_env curr prev) = Some abs.
+Proof.
+intros curr prev x Hcurr Hprev. unfold hold_env.
+rewrite PositiveMap.gmapi, Hcurr. simpl. now rewrite Hprev.
+Qed. 
+
+Lemma hold_env_never_None : forall (curr prev : venv) (x : ident),
+  PositiveMap.find x (hold_env curr prev) = None <-> PositiveMap.find x curr = None.
+Proof.
+intros curr prev x. unfold hold_env. rewrite PositiveMap.gmapi.
+split; intro Heq.
+- destruct (PositiveMap.find x curr); trivial. discriminate.
+- now rewrite Heq.
+Qed.
+
+Lemma hold_env_abs : forall (curr prev : venv) (x : ident),
+  PositiveMap.find x (hold_env curr prev) = Some abs -> PositiveMap.find x curr = Some abs.
+Proof.
+intros curr prev x Hin. unfold hold_env in Hin. rewrite PositiveMap.gmapi in Hin.
+destruct (PositiveMap.find x curr) as [[| v] |]; trivial.
+Qed.
+
+Lemma hold_env_abs_spec : forall (curr prev : venv) (x : ident),
+  PositiveMap.find x (hold_env curr prev) = Some abs <->
+  PositiveMap.find x curr = Some abs /\ (PositiveMap.find x prev = Some abs \/ PositiveMap.find x prev = None).
+Proof.
+intros curr prev x. split; intro H.
++ split.
+  - eapply hold_env_abs. eassumption.
+  - destruct (PositiveMap.find x prev) as [[| v] |] eqn:Hin; intuition.
+    left. rewrite <- H. symmetry. apply hold_env_out; trivial. now apply hold_env_abs in H.
++ destruct H as [H1 [H2 | H2]].
+  - now apply hold_env_out.
+  - now apply hold_env_none.
+Qed.
+
+(** ***  All environments inside a given history have the same domain  **)
+
+(** First, we need to check that the domain of all environment in the history is the same.
+    This property is preversed by hold. *)
+Definition same_dom (env1 env2 : venv) := forall x : ident, PositiveMap.In x env1 <-> PositiveMap.In x env2.
+
+Instance same_dom_equiv : Equivalence same_dom.
+Proof. unfold same_dom. split.
++ intros ? ?. reflexivity.
++ intros e e' ? ?. symmetry. auto.
++ intros e e' e'' H H' ?. now rewrite H.
+Qed.
+
+Definition history_valid (h : history) :=
+  match h with
+    | nil => True
+    | env0 :: h => List.Forall (same_dom env0) h
+  end.
+
+Lemma hold_env_dom_valid : forall curr prev, same_dom (hold_env curr prev) curr.
+Proof.
+intros curr prev x. split; intros [[| v] Hin].
++ exists abs. eapply PositiveMap.find_2, hold_env_abs, PositiveMap.find_1. eassumption.
++ apply PositiveMap.find_1 in Hin.
+  destruct (PositiveMap.find x curr) as [v' |] eqn:Hcurr.
+  - exists v'. now apply PositiveMap.find_2.
+  - rewrite <- hold_env_never_None in Hcurr. rewrite Hcurr in Hin. discriminate.
++ apply PositiveMap.find_1 in Hin.
+  destruct (PositiveMap.find x prev) as [v |] eqn:Hprev.
+  - exists v. apply PositiveMap.find_2. now apply hold_env_out.
+  - exists abs. apply PositiveMap.find_2. now apply hold_env_none.
++ exists v. apply PositiveMap.find_2. now apply hold_env_in.
+Qed.
+
+Lemma hold_history_valid : forall h, history_valid (hold h) <-> history_valid h.
+Proof.
+intros h. destruct h as [| env h]; try now intuition.
+simpl.
+assert (HP : forall l env e, Forall (same_dom (hold_env env e)) l <-> Forall (same_dom env) l).
+{ intros ? ? ?. apply Forall_compat; trivial. repeat intro; subst. now rewrite hold_env_dom_valid. }
+rewrite HP.
+induction h as [| env1 h]; try now split; constructor.
+split; intro Hvalid.
++ simpl. inversion_clear Hvalid. constructor.
+  - now rewrite hold_env_dom_valid in H.
+  - now rewrite <- IHh.
++ simpl. inversion_clear Hvalid. constructor.
+  - now rewrite hold_env_dom_valid.
+  - now rewrite IHh.
+Qed.
+
+Lemma history_valid_cons : forall env (h : history), history_valid (env :: h) -> history_valid h.
+Proof.
+intros env h H. destruct h as [| env1 h]; simpl in *; auto.
+cut (Forall (same_dom env) h).
+- apply Forall_compat; trivial. intros ? e ?; subst. inversion_clear H. now rewrite H0.
+- now inversion H.
+Qed.
+
+Lemma history_valid_dom : forall d n env h, n < S (length h) -> history_valid (env :: h) ->
+  same_dom (nth n (env :: h) d) env.
+Proof.
+intros d n env h Hn Hvalid. simpl in Hvalid. destruct n.
++ reflexivity.
++ simpl. rewrite Forall_forall in Hvalid. symmetry. apply Hvalid, nth_In. omega.
+Qed.
+
+Corollary history_valid_same_dom : forall d n n' (h : history), n < length h -> n' < length h -> history_valid h ->
+  same_dom (nth n h d) (nth n' h d).
+Proof.
+intros d n n' h Hn Hn' Hh. destruct h as [| env h].
+- destruct n, n'; reflexivity.
+- repeat rewrite history_valid_dom; auto. reflexivity.
+Qed.
+
+(** ***  Lemmas about [hold]  **)
+
+Lemma hold_length : forall h, length (hold h) = length h.
+Proof. intros h. induction h; simpl; auto. Qed.
+
+Lemma hold_in : forall (d : venv) (x : ident) n (h : history) v, n < length h ->
+  PositiveMap.find x (nth n h d) = Some (here v) ->
+  PositiveMap.find x (nth n (hold h) d) = Some (here v).
+Proof.
+intros d x n. induction n; intros h v Hn Hx; simpl.
+- destruct h; simpl in *; trivial. now apply hold_env_in.
+- destruct h; simpl in *; trivial. apply IHn; trivial. omega.
+Qed.
+
+Lemma hold_out_last : forall (d : venv) (x : ident) (h : history),
+  PositiveMap.find x (last h d) = Some abs ->
+  PositiveMap.find x (last (hold h) d) = Some abs.
+Proof.
+intros d x h Hx. induction h; trivial. destruct h.
+- simpl. apply hold_env_none; trivial. apply PositiveMap.gempty.
+- now apply IHh.
+Qed.
+
+Lemma hold_out : forall (d : venv) (x : ident) n (h : history), (S n) < length h -> history_valid h ->
+  PositiveMap.find x (nth n h d) = Some abs ->
+  PositiveMap.find x (nth n (hold h) d) = PositiveMap.find x (nth (S n) (hold h) d).
+Proof.
+intros d x n. induction n; intros h Hn Hh Hx.
++ induction h as [| env1 [| env2 h]]; trivial; simpl in Hn; try omega; [].
+  assert (Hin : PositiveMap.In x env2).
+  { inversion_clear Hh. rewrite <- (H x). exists abs. apply PositiveMap.find_2. assumption. }
+  destruct Hin as [[| v] Hin]. apply PositiveMap.find_1 in Hin.
+  - assert (Hin2 : PositiveMap.In x (hold_env env2 (hd (PositiveMap.empty value) (hold h)))).
+    { rewrite (hold_env_dom_valid env2 _ x). exists abs. now apply PositiveMap.find_2. }
+    destruct Hin2 as [v Hin2]. apply PositiveMap.find_1 in Hin2.
+    simpl in *. rewrite (@hold_env_out _ _ _ v); trivial. now symmetry.
+  - clear IHh. simpl nth at 1. rewrite (@hold_env_out _ _ _ v); trivial; [symmetry |];
+    apply (@hold_in d x 1 (env1 :: env2 :: h)); auto.
++ destruct h as [| env1 h]; simpl in *; trivial; [].
+  apply IHn; trivial.
+  - omega.
+  - eapply history_valid_cons. eassumption.
+Qed.
+
+Lemma hold_never_None : forall d (x : ident) n h,
+  PositiveMap.find x (nth n (hold h) d) = None <-> PositiveMap.find x (nth n h d) = None.
+Proof.
+intros d x n. induction n; intro h.
+- destruct h as [| env h]; simpl; try reflexivity. apply hold_env_never_None.
+- destruct h as [| env h]; simpl; try reflexivity. apply IHn.
+Qed.
+
+Lemma hold_abs_next : forall d (x : ident) n (h : history), S n < length h -> history_valid h ->
+  PositiveMap.find x (nth n (hold h) d) = Some abs -> PositiveMap.find x (nth (S n) (hold h) d) = Some abs.
+Proof.
+intros d x n. induction n; intros h Hn Hvalid Hx.
+- destruct h as [| env h]; simpl in Hn; try omega.
+  assert (Hnow := hold_env_abs _ _ _ Hx). now rewrite <- hold_out.
+- destruct h as [| env h]; simpl in Hn; try omega. simpl.
+  apply IHn; trivial; try omega. eapply history_valid_cons. eassumption.
+Qed.
+
+Corollary hold_abs_rec : forall d (x : ident) n m (h : history), n + m < length h -> history_valid h ->
+  PositiveMap.find x (nth n (hold h) d) = Some abs -> PositiveMap.find x (nth (n + m) (hold h) d) = Some abs.
+Proof.
+intros d x n m. induction m; intros.
+- now rewrite <- plus_n_O.
+- rewrite <- plus_n_Sm in *. apply hold_abs_next; trivial. apply IHm; trivial. omega.
+Qed.
+
+Lemma hold_abs : forall d (x : ident) n (h : history), n < length h -> history_valid h ->
+  PositiveMap.find x (nth n (hold h) d) = Some abs -> PositiveMap.find x (nth n h d) = Some abs.
+Proof.
+intros d x n. induction n; intros h Hn Hvalid Hx.
+- destruct h as [| env h]; simpl in *; try omega.
+  now apply hold_env_abs in Hx.
+- destruct h as [| env h]; simpl in *; try omega.
+  apply IHn; trivial; try omega. eapply history_valid_cons. eassumption.
+Qed.
+
+Lemma hold_abs_spec : forall d (x : ident) (h : history) n, n < length h -> history_valid h ->
+  (PositiveMap.find x (nth n (hold h) d) = Some abs <->
+   forall m, n + m < length h -> PositiveMap.find x (nth (n + m) h d) = Some abs).
+Proof.
+intros d x h n Hn Hvalid. split; intro H.
+* intros. apply hold_abs; trivial. now apply hold_abs_rec.
+* revert h Hn Hvalid H. induction n; intros h Hn Hvalid H.
+  + simpl in H. induction h as [| env h].
+    - simpl in Hn. omega.
+    - { assert (Henv : PositiveMap.find x env = Some abs). { apply (H 0). simpl. omega. }
+        destruct h as [| env' h]; simpl.
+        + apply hold_env_none; trivial. rewrite find_None_not_In.
+          intros [v Habs]. revert Habs. apply PositiveMap.empty_1.
+        + apply hold_env_out; trivial. apply IHh.
+          - simpl. omega.
+          - eapply history_valid_cons. eassumption.
+          - intros m hm. apply (H (S m)). simpl in *. omega. }
+  + destruct h as [| env h]; simpl in Hn; try omega.
+    simpl. apply IHn.
+    - omega.
+    - eapply history_valid_cons. eassumption.
+    - intros. apply H. simpl. omega.
+Qed.
+
+(** The full specification of [hold] *)
+Theorem hold_spec : forall d x n h v, history_valid h -> n < length h ->
+  (PositiveMap.find x (nth n (hold h) d) = Some (here v) <->
+   exists n', n + n' < length h
+           /\ PositiveMap.find x (nth (n + n') h d) = Some (here v)
+           /\ forall m, m < n' -> PositiveMap.find x (nth (n + m) h d) = Some abs).
+Proof.
+intros d x n. induction n; intros h v Hvalid Hn.
+* simpl plus. induction h as [| env h]; simpl in Hn; try omega.
+  destruct (PositiveMap.find x env) as [[| vx] |] eqn:Henv.
+  + (** [x] is [abs] in [env] *)
+    destruct h as [| env' h].
+    - { simpl. split; intro Habs.
+        + exfalso. cut (Some (here v) = Some abs). discriminate.
+          rewrite <- Habs. apply hold_env_none; trivial. rewrite find_None_not_In.
+          intros [? Hin]. apply (PositiveMap.empty_1 Hin).
+        + destruct Habs as [[| ?] [? [Henv' _]]]; try omega.
+          rewrite Henv in Henv'. discriminate. }
+    - { change env with (nth 0 (env :: env' :: h) d) in Henv.
+        assert (Hlen : 1 < length (env :: env' :: h)) by (simpl; omega).
+        rewrite (hold_out _ _ _ Hlen Hvalid Henv); trivial; try (simpl; omega); []. simpl.
+        rewrite IHh.
+        * split; intros [n [Hn' [Hmax Hlt]]].
+          + exists (S n). simpl in *. repeat split; trivial; try omega.
+            intros [| m] Hm; trivial. apply Hlt. omega.
+          + simpl in Henv. destruct n.
+            - rewrite Henv in Hmax. discriminate.
+            - exists n. simpl. repeat split; trivial; try omega.
+              intros m Hm. apply (Hlt (S m)). omega.
+        * now apply history_valid_cons in Hvalid.
+        * simpl. omega. }
+  + (** [x] is [here vx] in [env] *)
+    simpl hold. simpl nth at 1. rewrite (hold_env_in _ _ _ Henv).
+    split; intro H.
+    - inv H. exists 0. simpl. repeat split; trivial. intros. omega.
+    - destruct H as [n [Hok [Hmax Hlt]]].
+      assert (n = 0).
+      { destruct n; trivial. exfalso.
+        cut (Some (here vx) = Some abs). discriminate.
+        rewrite <- Henv. apply (Hlt 0). omega. }
+      subst. simpl in Hmax. now rewrite Henv in Hmax.
+  + (** [x] is not present in [h] *)
+    rewrite find_None_not_In in Henv.
+    split; intro H.
+    - elim Henv. erewrite <- (hold_env_dom_valid _ _ x).
+      exists (here v). apply PositiveMap.find_2. simpl in *. eassumption.
+    - elim Henv. destruct H as [n [Hn' [Hin Hlt]]].
+      rewrite (@history_valid_same_dom d 0 n (env :: h) Hn Hn' Hvalid x).
+      exists (here v). now apply PositiveMap.find_2.
+* destruct h as [| env h]; simpl in Hn |- *; try omega.
+  setoid_rewrite <- NPeano.Nat.succ_lt_mono. apply IHn.
+  - now apply history_valid_cons in Hvalid.
+  - omega.
+Qed.
+
+Lemma hold_idempotent : forall x n h d, history_valid h ->
+  PositiveMap.find x (nth n (hold (hold h)) d) = PositiveMap.find x (nth n (hold h) d).
+Proof.
+intros x n. induction n; intro h.
+* induction h as [| env h]; intros d Hh.
+  + reflexivity.
+  + destruct (PositiveMap.find x env) as [[| v] |] eqn:Heq.
+    - { destruct h as [| env' h].
+        * simpl.
+          assert (H : PositiveMap.find x (hold_env env (PositiveMap.empty value)) = Some abs).
+          { apply hold_env_none; trivial. apply PositiveMap.gempty. }
+          rewrite H. apply hold_env_none; trivial. apply PositiveMap.gempty.
+        * destruct (PositiveMap.find x (nth 0 (hold (env :: env' :: h)) d)) as [[| v] |] eqn:Hhold.
+          + rewrite hold_abs_spec.
+            - intros. apply hold_abs_rec; trivial. now rewrite <- hold_length.
+            - rewrite hold_length. simpl. omega.
+            - now rewrite hold_history_valid.
+          + apply hold_in; trivial. simpl. omega.
+          + now rewrite hold_never_None. }
+    - { erewrite hold_in.
+        + symmetry. apply hold_in; simpl; omega || eassumption.
+        + rewrite hold_length. simpl. omega.
+        + apply hold_in; simpl; omega || eassumption. }
+    - assert (H : PositiveMap.find x (nth 0 (hold (env :: h)) d) = None) by now rewrite hold_never_None.
+      rewrite H. now rewrite hold_never_None.
+* intros d Hh. destruct h as [| env h]; simpl.
+  + reflexivity.
+  + apply IHn. now apply history_valid_cons in Hh.
+Qed.
+
+(** **  The equivalence of [fby] with and without [hold]  **)
+
+(** The specification of [fby_rev] *)
+Lemma fby_aux_snd_spec : forall v0 v vl, snd (fby_aux v0 vl) = v <->
+  (exists n, nth n vl abs = here v /\ forall m, m < n -> nth m vl abs = abs)
+  \/ v = v0 /\ forall n, nth n vl abs = abs.
+Proof.
+intros v0 v vl. revert v0. induction vl as [| v1 vl]; intros v0.
+* setoid_rewrite nth_nil. simpl. split; intro H.
+  + subst. auto.
+  + destruct H as [[? [? _]] | [? _]]; discriminate || auto.
+* split; intro H.
+  + destruct v1 as [| v1]; simpl in H.
+    - { destruct (fby_aux v0 vl) eqn:Hfby. simpl in H. subst.
+        specialize (IHvl v0). rewrite Hfby in IHvl.
+        assert (Hrec : v = v) by reflexivity. rewrite IHvl in Hrec. clear IHvl.
+        destruct Hrec as [[n [Hn Hother]] | [Hn Hother]].
+        + left. exists (S n). simpl. split; trivial.
+          intros [| m] Hlt; trivial. apply Hother. omega.
+        + right. split; trivial. intros [| n]; trivial. apply Hother. }
+    - destruct (fby_aux v0 vl) eqn:Hfby. simpl in H. subst v.
+      specialize (IHvl v1). left. exists 0. split; trivial. intros. omega.
+  + destruct v1 as [| v1]; simpl.
+    - { destruct (fby_aux v0 vl) eqn:Hfby. change (snd (l, c) = v). rewrite <- Hfby.
+        rewrite IHvl. clear IHvl. destruct H as [[[| n] [Hn Hother]] | [Hn Hother]].
+        + discriminate.
+        + left. exists n. simpl. split; trivial. intros m Hlt. apply (Hother (S m)). omega.
+        + right. split; trivial. intro n. apply (Hother (S n)). }
+    - { destruct (fby_aux v0 vl) eqn:Hfby. simpl.
+        destruct H as [[n [Hn Hother]] | [Hn Hother]].
+        + assert (n = 0).
+          { destruct n; trivial. exfalso. cut (here v1 = abs). discriminate.
+            rewrite <- (Hother 0); trivial. omega. }
+          subst. simpl in Hn. now inv Hn.
+        + exfalso. cut (here v1 = abs). discriminate.
+          now rewrite <- (Hother 0). }
+Qed.
+
+Theorem fby_rev_spec : forall n v0 v vl, nth n (fby_rev v0 vl) abs = here v
+  <-> nth n vl abs <> abs
+   /\ ((exists n', nth (S (n + n')) vl abs = here v /\ forall m, m < n' -> nth (S (n + m)) vl abs = abs)
+       \/ v = v0 /\ forall n', nth (S (n + n')) vl abs = abs).
+Proof.
+intro n. induction n; intros v0 v vl.
+* simpl plus. unfold fby_rev. destruct vl as [| [| v1] vl]; simpl.
+  + intuition discriminate.
+  + destruct (fby_aux v0 vl); simpl. intuition discriminate.
+  + destruct (fby_aux v0 vl) eqn:Hfby; simpl.
+    assert (Hequiv : here c = here v <-> c = v). { split; intro Heq; subst; trivial. now injection Heq. }
+    rewrite Hequiv. change c with (snd (l, c)). rewrite <- Hfby.
+    rewrite fby_aux_snd_spec. intuition discriminate.
+* destruct vl; simpl.
+  + split; intro Habs.
+    - discriminate.
+    - destruct Habs as [Habs _]. now elim Habs.
+  + rewrite fby_rev_next. apply IHn.
+Qed.
+
+Lemma sem_var_length : forall h x vl, sem_var h x vl -> length vl = length h.
+Proof. unfold sem_var. intros h x vl Hvar. now rewrite <- (map_length (@Some value)), <- Hvar, map_length. Qed.
+
+Lemma sem_var_cons : forall env h x v vl, sem_var (env :: h) x (v :: vl) -> sem_var h x vl.
+Proof. unfold sem_var. intros * Hsem. now inversion Hsem. Qed.
+
+Lemma sem_var_nth : forall n h x vl, sem_var h x vl -> n < length h ->
+  PositiveMap.find x (nth n h (PositiveMap.empty _)) = Some (nth n vl abs).
+Proof.
+intros n h x vl Hsem.
+assert (Hlen := sem_var_length Hsem).
+revert h x vl Hsem Hlen. induction n; intros h x vl Hsem Hlen Hn.
++ destruct vl as [| v vl], h as [| env h]; try discriminate.
+  - simpl in Hn. omega.
+  - unfold sem_var in *. simpl in *. now inversion Hsem.
++ destruct vl as [| v vl], h as [| env h]; try discriminate.
+  - simpl in Hn. omega.
+  - simpl in *. apply IHn; try omega. apply (sem_var_cons Hsem).
+Qed.
+
+(* General equivalence except for the first instant. *)
+Theorem fby_equivalence : forall h x vl1 vl2, history_valid h ->
+  sem_var h x vl1 -> sem_var (hold h) x vl2 ->
+  forall n v0 v, S n < length h -> ~(forall m, nth (S n + m) vl1 abs = abs) ->
+                 nth n (fby_rev v0 vl1) abs = here v -> nth (S n) vl2 abs = here v.
+Proof.
+intros h x vl1 vl2 Hvalid Husual Hhold n v0 v Hn Hnext Hv.
+assert (Hlen : length vl1 = length vl2).
+{ rewrite (sem_var_length Husual), (sem_var_length Hhold), hold_length. reflexivity. }
+cut (Some (nth (S n) vl2 abs) = Some (here v)); try now intro H; injection H.
+assert (S n < length (hold h)) by now rewrite hold_length.
+rewrite <- (sem_var_nth Hhold); trivial.
+rewrite hold_spec; trivial.
+simpl plus. rewrite fby_rev_spec in Hv.
+destruct Hv as [Hnow [[n' [Hmax Hlt]] | [Heq Hall]]]; try contradiction.
+assert (S (n + n') < length h).
+{ rewrite <- (sem_var_length Husual). apply (@nth_not_default_lt_length _ abs). now rewrite Hmax. }
+exists n'. repeat split.
++ assumption.
++ rewrite (sem_var_nth Husual).
+  - now rewrite Hmax.
+  - assumption.
++ intros. rewrite (sem_var_nth Husual); try omega. now rewrite Hlt.
+Qed.
+
+(* The theorem for the first non [abs] instant. *)
+Theorem fby_non_equiv_first : forall h x vl1 vl2, history_valid h ->
+  sem_var h x vl1 -> sem_var (hold h) x vl2 ->
+  forall n v0 v, S n < length h -> (forall m, nth (S n + m) vl1 abs = abs) ->
+                 nth n (fby_rev v0 vl1) abs = here v -> nth (S n) vl2 abs = abs.
+Proof.
+intros h x vl1 vl2 Hvalid Husual Hhold n v0 v Hn Hlast Hv.
+cut (Some (nth (S n) vl2 abs) = Some abs). now intro H; injection H.
+rewrite <- (sem_var_nth Hhold).
+- rewrite hold_abs_spec; trivial.
+  intros m Hlt. rewrite (sem_var_nth Husual); trivial. f_equal. apply Hlast.
+- now rewrite hold_length.
+Qed.
+
+(** The more interesting result? *)
+Theorem fby_hold_equiv : forall h x vl, history_valid h -> sem_var (hold h) x vl ->
+  forall n v0 v, S n < length h -> ~(forall m, nth (S n + m) vl abs = abs) ->
+                 nth n (fby_rev v0 vl) abs = here v -> nth (S n) vl abs = here v.
+Proof.
+intros h x vl Hvalid Hh n v0 v Hn Hlast Hv.
+cut (Some (nth (S n) vl abs) = Some (here v)). now intro H; injection H.
+rewrite fby_rev_spec in Hv.
+destruct Hv as [Hnow [[m [Hmax Hlt]] | [? ?]]]; try contradiction.
+rewrite <- (sem_var_nth Hh).
+* rewrite <- hold_idempotent; trivial.
+  rewrite <- hold_history_valid in Hvalid. rewrite <- hold_length in Hn.
+  rewrite hold_spec; trivial. exists m. repeat split.
+  + rewrite <- (sem_var_length Hh).
+    apply (@nth_not_default_lt_length _ abs). simpl. erewrite Hmax. discriminate.
+  + assert (m = 0).
+    { destruct m; trivial. exfalso. apply Hlast. intro n'.
+      destruct (Compare_dec.le_lt_dec (length (hold h)) (S n + n')) as [Hn' | Hn'].
+      + apply nth_overflow. now rewrite (sem_var_length Hh).
+      + cut (Some (nth (S n + n') vl abs) = Some abs). now intro H; injection H.
+        rewrite <- (sem_var_nth Hh); trivial.
+        rewrite hold_length in Hn'. rewrite hold_history_valid in Hvalid.
+        rewrite hold_abs_rec; trivial. rewrite (sem_var_nth Hh); trivial.
+        f_equal. rewrite (plus_n_O n). apply Hlt. omega. }
+    subst m. clear Hlt. rewrite <- plus_n_O in *. erewrite sem_var_nth; try eassumption. now f_equal.
+  + intros m' Hm.
+    assert (Hneq : S n + m' < length h).
+    { assert (Hneq : here v <> abs) by discriminate. rewrite <- Hmax in Hneq.
+      apply nth_not_default_lt_length in Hneq.
+      rewrite <- hold_length, <- (sem_var_length Hh). omega. }
+    rewrite (sem_var_nth Hh).
+    - simpl. now rewrite Hlt.
+    - now rewrite hold_length.
+* now rewrite hold_length.
+Qed.
+
+
+(** Defining a new semantics for held histories would only require to
+    delete the first element and shift all elements by one after the first non [abs],
+    inseting the inital constant in its place.
+    Of course, if there are no such first element, we should return a list full of [abs]. *)
+
+(** Splits a list after its last non [abs] element.
+    The first component (if not None) is the list up to this last element, 
+    the second list contains the trailing [abs].
+    Provided we have a non [abs] element, then we can write
+    first res ++ second res = original list. *)
+
+Fixpoint split_last l : option (list value) * list value :=
+  match l with
+    | nil => (None, nil)
+    | abs :: l => match split_last l with
+                    | (None, l2) => (None, abs :: l2)
+                    | (Some l1, l2) => (Some (abs :: l1), l2)
+                  end
+    | here v :: l => match split_last l with
+                       | (None, l2) => (Some (here v :: nil), l2)
+                       | (Some l1, l2) => (Some (here v :: l1), l2)
+                     end
+  end.
+
+Lemma split_last_None : forall l l', split_last l = (None, l') <-> l = l' /\ l = alls abs l.
+Proof.
+intro l. induction l as [| [| e] l]; intro l'; simpl.
+* split; intro H.
+  + simpl in H. inversion_clear H. intuition.
+  + now destruct H; subst.
+* destruct (split_last l) as [[l1 |] l2].
+  + split; intro H.
+    - inversion H.
+    - destruct H as [? H']. subst. injection H'. intro H.
+      apply (conj (eq_refl l)) in H. rewrite <- IHl in H. discriminate.
+  + split; intro H.
+    - inversion_clear H. specialize (IHl l2). apply proj1 in IHl. specialize (IHl (reflexivity _)).
+      destruct IHl as [? IHl]. subst l2. now split; f_equal.
+    - f_equal. destruct H as [H1 H2]. subst. f_equal. injection H2. intro H.
+      apply (conj (eq_refl l)) in H. rewrite <- IHl in H. now inversion H.
+* destruct (split_last l) as [[l1 |] l2].
+  + split; intro H.
+    - inversion H.
+    - destruct H as [? H']. subst. inversion H'.
+  + split; intro H.
+    - inversion H.
+    - destruct H as [_ H]. inversion H.
+Qed.
+
+Lemma split_last_Some : forall l l1 l2, split_last l = (Some l1, l2) <-> 
+  l = l1 ++ l2 /\ (exists v, last l1 abs = here v) /\ l2 = alls abs l2.
+Proof.
+intro l. induction l as [| [| e] l]; intros l1 l2.
+* simpl. split; intro H.
+  + discriminate.
+  + destruct H as [H1 [H2 H3]]. destruct l1, l2; discriminate.
+* split; intro H; simpl in *.
+  + destruct (split_last l) as [[l1' |] l2'].
+    - destruct (proj1 (IHl l1' l2') (reflexivity _)) as [v [H1 H2]].
+      inv H. exists v. now split.
+    - inversion H.
+  + destruct H as [v [H1 H2]]. destruct l1 as [| ? l1]; try discriminate.
+    assert (Heq : split_last l = (Some l1, l2)). { rewrite IHl. exists v. inversion H1. now split. }
+    rewrite Heq. now inversion H1.
+* split; intro H; simpl in *.
+  + destruct (split_last l) as [[l1' |] l2'] eqn:Hsplit.
+    - inv H. destruct (proj1 (IHl l1' l2)) as [v [H1 H2]]; trivial.
+      exists v. split; trivial. now subst l.
+    - inv H. exists e. rewrite split_last_None in Hsplit. destruct Hsplit. subst l2. now split.
+  + destruct H as [v [H1 H2]]. destruct l1 as [| e1 l1].
+    - inversion_clear H1.
+      assert (Heq : split_last l2 = (None, l2)). { rewrite split_last_None. now split. }
+      now rewrite Heq.
+    - specialize (IHl l1 l2). inversion H1. subst l e1.
+      assert (Heq : split_last (l1 ++ here v :: l2) = (Some l1, l2)). { rewrite IHl. exists v. now split. }
+      now rewrite Heq.
+Qed.
+
+(** The simpler definition of [fby] with [hold]. *)
+Definition hold_fby_rev v vl := 
+  match vl with
+    | nil => nil
+    | _ :: vl => match split_last vl with
+                   | (None, l2) => vl
+                   | (Some l1, l2) => l1 ++ here v :: l2
+                 end
+  end.
+
+Inductive held_sem_equation_rev (G : global) : history -> equation -> Prop :=
+  | HSEqDef_rev : forall H x cae v,
+      sem_lexp H (Evar x) v -> sem_caexp H cae v -> held_sem_equation_rev G H (EqDef x cae)
+  | HSEqApp_rev : forall H x f arg input output eqs H' vi vo,
+      PositiveMap.find f G = Some (mk_node f input output eqs) ->
+      sem_laexp H arg vi ->
+      sem_lexp H (Evar x) vo ->
+      sem_lexp H' (Evar input.(v_name)) vi ->
+      sem_lexp H' (Evar output.(v_name)) vo ->
+      List.Forall (held_sem_equation_rev G H') eqs ->
+      held_sem_equation_rev G H (EqApp x f arg)
+  | HSEqFby_rev : forall H x v (y : var_dec) cl,
+      sem_var H y cl ->
+      sem_lexp H (Evar x) (hold_fby_rev v cl) ->
+      held_sem_equation_rev G H (EqFby x v y).
+
+Theorem hold_equivalence : forall G h eqn,
+  sem_equation_rev G h eqn <-> held_sem_equation_rev G (hold h) eqn.
+Proof.
+intros G h eqn.
+destruct eqn.
++ split; intro H.
+  - inversion_clear H. econstructor 1.
++ 
++ 
+Qed.
